\section{The quantized universal enveloping algebra $U_q(\sll(2))$}

$U_q(\sll(2))$ is a deformation of the universal enveloping algebra
$U(\sll(2))$ defined in \ref{UnivEnvAlg}, which in some sense approaches
$U(\sll(2))$ as $q \to 1$. In this section we will define $U_q(\sll(2))$ and
explain its relationship to $U(\sll(2))$.


Let $q$ be an indeterminate. $U_q(\sll(2))$ is the associative algebra over
$\mathbb{Q}(q)$ with generators $E,F,K, K^{-1}$ and relations 

\todo{should it be $\mathbb{Q}(q)$ or $\mathbb{C}(q)$?}
\begin{align}
    KK^{-1} &= 1 = K^{-1}K \\
    KEK^{-1} &= q^2 E \\
    KFK^{-1} &= q^{-2} F \\
    [E,F] &= \frac{K - K^{-1}}{q - q^{-1}}
\end{align}

% not sure if this is still useful:
%
% There is a unique algebra automorphism of $U_q(\sll(2))$ such that 
% \begin{equation}
%     \omega(E) = F, \omega(F) = E, \omega(K) = K^{-1}
% \end{equation}
% 
% This is called the \emph{Cartan automorphism}. We will use this later when
% constructing representations of $U_q(\sll(2))$.

Before proceeding, we will note some relations between the generators
$E,F,K,K^{-1}$ which will be useful later on. The following can be checked
easily by induction:

\begin{align}
    \label{EFrelations}
    EF^s = F^sE + [s]_q F^{s-1} \frac{Kq^{1-s} - K^{-1} q^{-(1-s)}}{q-q^{-1}} \\
    FE^s = E^sF - [s]_q E^{s-1} \frac{Kq^{s-1} - K^{-1} q^{-(s-1)}}{q-q^{-1}}
\end{align}

\section{A Hopf Algebra Structure on $U_q(\sll(2))$}
We can define a Hopf algebra structure on $U_q(\sll(2))$ as follows:

% from Kassel, p. 140
\begin{align}
    \Delta(E) &= 1 \otimes E + E \otimes K &  \Delta(F) &= K^{-1} \otimes F + F \otimes 1 \\
    \Delta(K) &= K \otimes K &  \Delta(K^{-1}) &= K^{-1} \otimes K^{-1}\\ 
    \varepsilon(E) &= \varepsilon(F) = 0 &  \varepsilon(K) &= \varepsilon(K^{-1}) = 1
\end{align}

and antipode defined by 

\begin{align}
    S(E) &= -EK^{-1} & S(F)      &= -KF \\
    S(K) &= K^{-1}   & S(K^{-1}) &= K 
\end{align}
It is straightforward to check that this defines a Hopf algebra structure. 

\section{Representations of $U_q(\sll(2))$}

The representation theory of $U_q(\sll(2))$ bears a striking resemblance to
that of $\sll(2)$. 

\begin{claim}
    Let $M$ be a finite dimensional $U_q(\sll(2))$-module. Then there is a
    vector $v \in M$ such that $Ev = 0$. 
\end{claim}

\todo{ do I need to prove that $K$ has eigenvectors?}

\begin{proof}
    Let $v_0$ be an eigenvector of $K$ with eigenvalue $\lambda$. $KEK^{-1} =
    q^2 E$, so it follows that $E^i v_0$ is an eigenvector of $K$ with
    eigenvalue $q^{2i}\lambda$. Each value $q^{2i}\lambda$ is different,
    therefore $K$ has infinitely many eigenvectors. 

    This is impossible, so some $E^i v_0$ must be zero.
\end{proof}

For any $\lambda \in k, \lambda \neq 0$ there is an infinite dimensional
$U_q(\sll(2))$-module $M(\lambda)$ with basis $v_0, v_1, v_2, \ldots$ such that
for any $i$,
\begin{align}
    Kv_i &= \lambda q^{-2i}v_i \\
    Fv_i &= v_{i+1} \\
    Ev_i &= \begin{cases} 0 & \text{if $i = 0$} \\
                          [i]_q \frac{\lambda q^{1-i} - \lambda^{-1}q^{i-1}}{q - q^{-1}}v_{i-1} & \text{else}
            \end{cases}
\end{align}

To see that this a $U_q(\sll(2))$-module, we can note that 

\todo{ set $U = U_q(\sll(2))$ here}

\begin{equation}
    M(\lambda) = U/(UE + U(K-\lambda))
\end{equation}

with $v_i$ being the coset of $F^i$. It follows from this that if $M$ is a
$U_q(\sll(2))$-module and $v \in M$ such that $Ev = 0$, $Kv = \lambda v$, there
is a unique homomorphism $\varphi: M(\lambda) \to M$ where $\varphi(v_0) = v$.
If $M$ is simple, then this homomorphism is surjective and it follows that $M$
is a quotient of $M(\lambda)$. 

We now have that 
\begin{claim}
    Any finite dimensional simple $U_q(\sll(2))$-module is a quotient of $M(\lambda)$.
\end{claim}

\begin{claim}
    $M(\lambda)$ is simple for $\lambda \neq \pm q^n$
\end{claim}

\begin{proof}
    See \cite{Jantzen1996}.
\end{proof}

For $\lambda = \pm q^{n}$, $M(\lambda)$ has one nontrivial submodule spanned by the $v_i$ with $i \geq n+1$.
This leads us to the following characterization (details can be found in \cite{Jantzen1996}):


For each integer $n \geq 0$, there are two unique (up to isomorphism)
representations of $U_q(\sll(2))$ of dimension $n+1$. 
The representations are $V(n,+)$ with basis $\left\{ v^+_0, \ldots, v^+_n
\right\}$ , and $V(n,-)$ with basis $\left\{ v^-_0, \ldots, v^-_n \right\}$
with action defined by 

% from Kassel, p. 101
\begin{align*}
    &K v^+_i = q^{n-2i} v^+_i  &
    &K v^-_i = -q^{n-2i} v^-_i \\
    &F v^+_i = \begin{cases} [i+1]_qv_{i+1}& \text{ if $i < n$} \\ 0& \text{ if $i = n$} \end{cases} &
    &F v^-_i = \begin{cases} [i+1]_qv'_{i+1}& \text{ if $i < n$} \\ 0& \text{ if $i = n$} \end{cases} \\
    &E v^+_i = \begin{cases} 
                     [n-i+1]_qv_{i-1}& \text{ if $i > 0$} \\ 
                    0& \text{ if $i = 0$} 
             \end{cases} &
    &E v^-_i = \begin{cases} 
                    -[n-i+1]_q v'_{i-1}& \text{ if $i > 0$} \\ 
                    0& \text{ if $i = 0$} 
             \end{cases}
\end{align*}

By the proof sketched above, these are the only representations of
$U_q(\sll(2))$. It is also possible to show that every finite dimensional
representation of $U_q(\sll(2))$ is semisimple. In other words, the category of
representations is semisimple.

\section{Representations of $U_q(\mathfrak{g})$}
    \subsection{$U_q(\mathfrak{g})$}

        % taken from Jantzen

        Let $\mathfrak{g}$ be an arbitrary semisimple algebra. Suppose $\Pi$ is
        a basis of the root system, and denote the entries of the Cartan matrix
        by 

        \begin{equation}
            a_{\alpha\beta} = 2(\alpha, \beta) / (\alpha, \alpha).
        \end{equation}

        Then the Lie algebra has a presentation with $3|\Pi|$ generators
        $x_\alpha, y_\alpha, h_\alpha$, $\alpha \in \Pi$ and the relations 

        \begin{align}
            \left[ h_\alpha, h_\beta \right] &= 0       &   \left[ x_\alpha, y_\beta \right] &= \delta_{\alpha\beta} h_\alpha \\
            \left[ h_\alpha, x_\beta \right] &= a_{\alpha\beta} x_\beta  &   \left[ h_\alpha, y_\beta \right] &= -a_{\alpha\beta} y_\beta \\
        \end{align}

        When constructing the algebra $U_q(\sll(2))$, we required that $q^2
        \neq 1$. We need a slightly stronger version of this in general: set

        \begin{equation}
            d_\alpha = \frac{(\alpha, \alpha)}{2}
        \end{equation}

        We require that $q^{2d_{\alpha}} \neq 0$ for all $\alpha$. This means
        that $q^2 \neq 0$, may also require that $q^4, q^6 \neq 0$, depending
        on the length of the longest root in $\mathfrak{g}$.

        Now set 

        \begin{equation}
            q_\alpha = q^{d_\alpha}
        \end{equation}

        and for $n \in \mathbf{Z}$,

        \begin{equation}
            [n]_\alpha = [n]_{q_\alpha} = \frac{q^{nd_\alpha} - q^{-nd_\alpha}}{q^{d_\alpha} - q^{-d_\alpha}}
        \end{equation}

        $[n]_\alpha^!$ and $\dbinom{n}{k}_\alpha$ are defined similarly: 
        
        \begin{equation}
            [n]_\alpha^! = [n]_{q_{\alpha}}^!
        \end{equation}
        \begin{equation}
            \dbinom{n}{k}_\alpha = \dbinom{n}{k}_{q_\alpha}
        \end{equation}

        \begin{defn}
            The quantized enveloping algebra $U_q(\mathfrak{g})$ has generators
            $E_\alpha, F_\alpha, K_\alpha, K_\alpha^{-1}$ for each $\alpha \in
            \Pi$, and relations

            \begin{align}
                K_\alpha K_\alpha^{-1} =\ &1  = K_\alpha^{-1}K_\alpha \\
                K_\alpha K_\beta &= K_\beta K_\alpha \\
                K_\alpha E_\beta K_\alpha^{-1} &= q^{(\alpha, \beta)} E_\beta \\
                K_\alpha F_\beta K_\alpha^{-1} &= q^{-(\alpha, \beta)} E_\beta \\
                [E_\alpha, F_\beta] &= \delta_{\alpha\beta} \frac{K_\alpha - K_\alpha^{-1}}{ q_\alpha - q_\alpha^{-1}} 
            \end{align}

            for all $\alpha, \beta \in \Pi$, and for $a \neq \beta$

            \begin{align}
                \sum_{s=0}^{1-a_{\alpha\beta}} (-1)^s \dbinom{1-a_{\alpha\beta}}{s}_\alpha E_\alpha^{1-a_{\alpha\beta} - s} E_\beta E_\alpha^s  &= 0 \\
                \sum_{s=0}^{1-a_{\alpha\beta}} (-1)^s \dbinom{1-a_{\alpha\beta}}{s}_\alpha F_\alpha^{1-a_{\alpha\beta} - s} F_\beta F_\alpha^s  &= 0 
            \end{align}
        \end{defn}
        \subsection{A Hopf algebra structure on $U_q(\mathfrak{g})$}

        We can define a Hopf algebra structure $(\Delta, \varepsilon, S)$ such
        that for all $\alpha \in \Pi$,

        \begin{align}
            \Delta(E_\alpha) &= E_\alpha \otimes 1 + K_\alpha \otimes E_\alpha      & \varepsilon(E_\alpha) &= 0  & S(E_\alpha) &= -K_\alpha^{-1} E_\alpha \\
            \Delta(F_\alpha) &= F_\alpha \otimes K_\alpha^{-1} + 1 \otimes F_\alpha & \varepsilon(F_\alpha) &= 0  & S(F_\alpha) &= -F_\alpha K_\alpha \\
            \Delta(K_\alpha) &= K_\alpha \otimes K_\alpha                           & \varepsilon(K_\alpha) &= 1  & S(K_\alpha) &= K_\alpha^{-1}
        \end{align}
    \subsection{Representation theory of $U_q(\mathfrak{g})$}


